\documentclass{article}
\usepackage{mathtools}
\usepackage{multicol}
\usepackage{setspace}
\usepackage[utf8]{inputenc}
\usepackage{fancyhdr}
\usepackage{tabularx}
\usepackage[american]{babel}
\usepackage{lipsum}


\usepackage[letterpaper,left=3cm,right=2cm,top=2.5cm,bottom=1.5cm]{geometry}
\onehalfspacing

\author{Pedro G\'{o}mez Mart\'{i}n}
\date{\today}
\title{Module 3 Review Assignment}

\begin{document}
\maketitle
\section{}
	\begin{align*}
		a_n=&\frac{\left(1+n\right)!}{n!}\\
		a_n=&\frac{\left(n+1\right)\left(n\right)\left(n-1\right)\cdots}{\left(n\right)\left(n-1\right)\cdots}\\
		a_n=&n+1\\
		&\lim\limits_{\infty}{\left[n+1\right]}=\infty\\
	\end{align*}
	
\section{}
	\begin{align*}
		\sum\limits_{n=0}^{\infty}&{\frac{\left(-2\right)^{n+3}}{5^{n+2}}}\\
		\sum\limits_{n=0}^{\infty}&{\frac{\left(-2\right)^{n}\left(-2\right)^3}{5^n{\left(5\right)^2}}}\\
		\frac{\left(-2\right)^3}{\left(5\right)^2}\sum\limits_{n=0}^{\infty}&\left(\frac{-2}{5}\right)^n\\
		-\frac{8}{25}\sum\limits_{n=0}^{\infty}&\left(-1\right)^n\left(\frac{2}{5}\right)^n\\
		-\frac{8}{25}\cdot\frac{5}{7}&=\fbox{$-\frac{40}{175}$}
	\end{align*}
	
\section{}
	\begin{align*}
		\sum\limits_{n=1}^{\infty}\frac{1}{n\left(n+2\right)} \rightarrow \frac{A}{n}+\frac{B}{n+2}=\frac{1}{n(n+2)} \rightarrow A(n+2)+Bn=1\ \Rightarrow\ A=\frac{1}{2}\ B=-\frac{1}{2}\\
		\frac{1}{2}\lim\limits_{N\rightarrow \infty}\left[\sum\limits_{n=0}^{N}\left(\frac{1}{n+2}-\frac{1}{n}\right) \right]=\frac{1}{2}\left(1+\frac{1}{2}+\lim\limits_{N\rightarrow \infty}\left[\frac{1}{N+2}\right]\right)=\frac{3}{4}
	\end{align*}
	
\section{}
	\begin{align*}
		\sum\limits_{n=1}^{\infty}\frac{(-1)^{n+1}(n+2\cdot 3^n)}{2^{2n+1}}=\sum\limits_{n=1}^{\infty}{\frac{(-1)^{n}(-1)(n+2)\cdot 3^n}{2^{2n}\cdot 2}}=\frac{1}{2} \sum\limits_{n=1}^{\infty}(-1)^n\frac{(n+2)\cdot 3^n}{2^{2n}}\\
		\lim\limits_{n\rightarrow \infty}\frac{(n+2\cdot 3^{n})}{2^{2n}}=0
	\end{align*}
	\begin{multicols}{2}
		\setlength{\columnseprule}{0.4pt}
		\begin{align*}
			\frac{(1+2)3}{2^2}\ \frac{(2+2)3^2}{2^4}
		\end{align*}
		\begin{align*}
			\frac{9}{4}&\ \frac{\not 4 \cdot 9}{\not 4 \cdot 4}&\ \frac{(3+2)3^3}{2^6}=\frac{5\cdot 27}{64}=\frac{135}{64}& \\
			b_1&\ b_2&\ b_3&
		\end{align*}
		\vfill
		\columnbreak
		\begin{align*}
			a_n&=\frac{\left(-1\right)^{n+1}\left(n+2\right)3^n}{2^{2n}}\\
			b_n&=\frac{\left(n+2\right)3^n}{2^{2n}}
		\end{align*}
		$a_1$ cancels $a_2$ and from $a_3$ on, $b_n$ converges.
	\end{multicols}
	
\section{}
	\begin{multicols}{3}
		\setlength{\columnseprule}{0.4pt}
		$\left.a\right)\ \sum\limits_{n=1}^{\infty}\left(\sqrt{2}\right)^{n}$\\
		geometric series\\
		$r=\sqrt{2}$\\
		$\left|r\right|>1$\\
		the series diverges by the nth term test
		\vfill\columnbreak
		$\left.b\right) \sum\limits_{n=1}^{\infty}\frac{\sqrt{n}}{n^2+\ln{\left(n\right)}}$\\
		$\lim\limits_{n\rightarrow \infty}\left[\frac{n^{\frac{1}{2}}}{n^2} : \frac{1}{n^2}\right]$\\
		$\lim\limits_{n\rightarrow \infty}\left[\frac{n^{\frac{1}{2}+2}}{n^2}\right]\rightarrow$ By the limit comparison test, both converge\\
		and by direct comparison test $\sum\limits_{n=1}^{\infty}{\frac{\sqrt{n}}{n^2+\ln{\left(n\right)}}}$ converges absolutely.
		\vfill\columnbreak
		$\sum\limits_{n=1}^{\infty}{e^{-1}n!}=\sum\limits_{n=1}^{\infty}{\frac{n!}{e^n}}$\\
		$\lim\limits_{n\rightarrow \infty}\left[\sqrt[n]{\left|\frac{n!}{e^n}\right|}\right]=\infty$\\
		by the Root test $\sum\limits_{n=1}^{\infty}{e^{-1}n!}$ diverges.
	\end{multicols}

\section{}
	\begin{multicols}{2}
		\begin{align*}
			\left.a\right)\ &\sum\limits_{n=1}^{\infty}{\left(\frac{1}{3}\right)^n}\\
			&\text{converges}\\
			&\left|r\right|<1
		\end{align*}
		\vfill\columnbreak
		\begin{align*}
			\left.b\right)\ 
			\sum\limits_{n=1}^{\infty}{\frac{1}{\ln{n}}}
			\fbox{$\frac{1}{\ln{n}}>\frac{1}{n}$}
		\end{align*}
		by direct comparison test, $a_n>b_n$ the series diverges
	\end{multicols}
	\begin{align*}
		\left.c\right)\ \sum\limits_{n=1}^{\infty}{\frac{2n}{n+1}}\ \ \ \frac{2(n+1)}{(n+1)+1}: \frac{2n}{n+1}\rightarrow \frac{\not 2 (n+1)^2}{\not 2 n(n+2)}=\frac{(n+1)^2}{n^2+2n}
	\end{align*}
	$\sum\limits_{n=1}^{\infty}{\frac{2n}{n+1}}$ diverges by the nth term test
	\begin{align*}
		\lim\limits_{n\rightarrow \infty}\left[\frac{(n+1)^2}{n^2+2n}\right]=1\ 1\not=0
	\end{align*}
	$\left.d\right)\ \sum\limits_{n=1}^{\infty}{\left(-1\right)}^n\frac{1}{\ln(n)}$ by the alternating series test, the series converge conditionally.\\
	$\left.e\right)\ \sum\limits_{n=1}^{\infty}\frac{1}{n(2n+1)}$ Converges by direct comparison to $\sum\limits_{n=1}^{\infty}{\frac{1}{n^2}}$
	
\section{}	
	\begin{align*}
		\sum\limits_{n=1}^{4}{\left(-1\right)^{n+1}\left(\frac{1}{2}\right)^n}=S_n
	\end{align*}
	$\left.a\right)\ S_4 = +\left(\frac{1}{2}\right)-\left(\frac{1}{4}\right)+\left(\frac{1}{8}\right)-\left(\frac{1}{16}\right) = \frac{4+1}{8}-\frac{4+1}{16} = \frac{10-5}{16} = \frac{5}{16}$\\
	$\left.b\right) \frac{5}{16}<S_n<\frac{11}{32}$\\
	$\left.c\right)\ \frac{\frac{1}{2}}{1-\left(\frac{1}{2}\right)}\cdot \frac{1}{2}=\frac{1}{2}$\\
	$\left.d\right)$ yes
	
\section{}
	\begin{multicols}{4}
		$\left.a\right)$ F\\
		\vfill\columnbreak
		$\left.b\right)$ F\\
		\vfill\columnbreak
		$\left.c\right)$ T\\
		\vfill\columnbreak
		$\left.d\right)$ T
	\end{multicols}
	
\section{}
	\begin{align*}
		\left.a\right)&\ \sum\limits_{n=0}^{\infty}{\frac{x^n}{3n+1}}\ \ \ \frac{\frac{x^{n+1}}{3\left(n+1\right)+1}}{\frac{x^n}{3n+1}}\\
		&\lim\limits_{n\rightarrow \infty}\left|\frac{x^{n+1}\left(3n+1\right)}{\left(3\left(n+1\right)\right)x^n}\right| = \lim\limits_{n\rightarrow \infty}\left|\frac{x\left(3n+1\right)}{3n+4}\right| = \lim\limits_{n\rightarrow \infty}\left[\left|x\right|\frac{3+\frac{1}{n}}{3+\frac{4}{n}}\right] = \left|x\right|\ \ \ -1<x<1
	\end{align*}
	
\end{document}
